Stopped at CTR

SafeSpawns.v
@@ -1,3 +1,4 @@
+From Elo Require Import Util.
 From Elo Require Import Core.
 
 (* ------------------------------------------------------------------------- *)
@@ -5,49 +6,49 @@ From Elo Require Import Core.
 (* ------------------------------------------------------------------------- *)
 
 (* A term is no-mut if it has no mutable references. *)
-Inductive NoMut : tm -> Prop :=
+Inductive no_mut : tm -> Prop :=
   | nomut_unit :
-    NoMut <{unit}>
+    no_mut <{unit}>
 
   | nomut_num : forall n,
-    NoMut <{N n}>
+    no_mut <{N n}>
 
-  | nomut_refI : forall ad T,
-    NoMut <{&ad :: i&T}>
+  | nomut_ad : forall ad T,
+    no_mut <{&ad :: i&T}>
 
   | nomut_new : forall T t,
-    NoMut t ->
-    NoMut <{new T t}>
+    no_mut t ->
+    no_mut <{new T t}>
 
   | nomut_load : forall t,
-    NoMut t ->
-    NoMut <{*t}>
+    no_mut t ->
+    no_mut <{*t}>
 
   | nomut_asg : forall t1 t2,
-    NoMut t1 ->
-    NoMut t2 ->
-    NoMut <{t1 = t2}>
+    no_mut t1 ->
+    no_mut t2 ->
+    no_mut <{t1 = t2}>
 
   | nomut_var : forall x,
-    NoMut <{var x}>
+    no_mut <{var x}>
 
   | nomut_fun : forall x Tx t,
-    NoMut t ->
-    NoMut <{fn x Tx t}>
+    no_mut t ->
+    no_mut <{fn x Tx t}>
 
   | nomut_call : forall t1 t2,
-    NoMut t1 ->
-    NoMut t2 ->
-    NoMut <{call t1 t2}>
+    no_mut t1 ->
+    no_mut t2 ->
+    no_mut <{call t1 t2}>
 
   | nomut_seq : forall t1 t2,
-    NoMut t1 ->
-    NoMut t2 ->
-    NoMut <{t1; t2}>
+    no_mut t1 ->
+    no_mut t2 ->
+    no_mut <{t1; t2}>
 
   | nomut_spawn : forall t,
-    NoMut t ->
-    NoMut <{spawn t}>
+    no_mut t ->
+    no_mut <{spawn t}>
   .
 
 (* ------------------------------------------------------------------------- *)
@@ -55,327 +56,171 @@ Inductive NoMut : tm -> Prop :=
 (* ------------------------------------------------------------------------- *)
 
 (* A term has safe spawns if all of its spawns have no mutable references. *)
-Inductive SafeSpawns : tm -> Prop :=
+Inductive safe_spawns : tm -> Prop :=
   | ss_unit :
-      SafeSpawns <{unit}>
+      safe_spawns <{unit}>
 
   | ss_num : forall n,
-      SafeSpawns <{N n}>
+      safe_spawns <{N n}>
 
-  | ss_ref : forall ad T,
-      SafeSpawns <{&ad :: T}>
+  | ss_ad : forall ad T,
+      safe_spawns <{&ad :: T}>
 
   | ss_new : forall T t,
-      SafeSpawns t ->
-      SafeSpawns <{new T t}>
+      safe_spawns t ->
+      safe_spawns <{new T t}>
 
   | ss_load : forall t,
-      SafeSpawns t ->
-      SafeSpawns <{*t}>
+      safe_spawns t ->
+      safe_spawns <{*t}>
 
   | ss_asg : forall t1 t2,
-      SafeSpawns t1 ->
-      SafeSpawns t2 ->
-      SafeSpawns <{t1 = t2}>
+      safe_spawns t1 ->
+      safe_spawns t2 ->
+      safe_spawns <{t1 = t2}>
 
   | ss_var : forall x,
-      SafeSpawns <{var x}>
+      safe_spawns <{var x}>
 
   | ss_fun : forall x Tx t,
-      SafeSpawns t ->
-      SafeSpawns <{fn x Tx t}>
+      safe_spawns t ->
+      safe_spawns <{fn x Tx t}>
 
   | ss_call : forall t1 t2,
-      SafeSpawns t1 ->
-      SafeSpawns t2 ->
-      SafeSpawns <{call t1 t2}>
+      safe_spawns t1 ->
+      safe_spawns t2 ->
+      safe_spawns <{call t1 t2}>
 
   | ss_seq : forall t1 t2,
-      SafeSpawns t1 ->
-      SafeSpawns t2 ->
-      SafeSpawns <{t1; t2}>
+      safe_spawns t1 ->
+      safe_spawns t2 ->
+      safe_spawns <{t1; t2}>
 
   | ss_spawn : forall t,
-      NoMut t ->
-      SafeSpawns <{spawn t}>
+      no_mut t ->
+      safe_spawns <{spawn t}>
   .
 
 (* ------------------------------------------------------------------------- *)
 (* has-var                                                                   *)
 (* ------------------------------------------------------------------------- *)
 
-Inductive HasVar (x : id) : tm  -> Prop :=
+Inductive has_var (x : id) : tm  -> Prop :=
   | hasvar_new : forall T t,
-      HasVar x t ->
-      HasVar x <{new T t}>
+      has_var x t ->
+      has_var x <{new T t}>
 
   | hasvar_load : forall t,
-      HasVar x t ->
-      HasVar x <{*t}>
+      has_var x t ->
+      has_var x <{*t}>
 
   | hasvar_asg1 : forall t1 t2,
-      HasVar x t1 ->
-      HasVar x <{t1 = t2}>
+      has_var x t1 ->
+      has_var x <{t1 = t2}>
 
   | hasvar_asg2 : forall t1 t2,
-      HasVar x t2 ->
-      HasVar x <{t1 = t2}>
+      has_var x t2 ->
+      has_var x <{t1 = t2}>
 
   | hasvar_var :
-      HasVar x <{var x}>
+      has_var x <{var x}>
 
   | hasvar_fun : forall x' Tx t,
       x <> x' ->
-      HasVar x t ->
-      HasVar x <{fn x' Tx t}>
+      has_var x t ->
+      has_var x <{fn x' Tx t}>
 
   | hasvar_call1 : forall t1 t2,
-      HasVar x t1 ->
-      HasVar x <{call t1 t2}>
+      has_var x t1 ->
+      has_var x <{call t1 t2}>
 
   | hasvar_call2 : forall t1 t2,
-      HasVar x t2 ->
-      HasVar x <{call t1 t2}>
+      has_var x t2 ->
+      has_var x <{call t1 t2}>
 
   | hasvar_seq1 : forall t1 t2,
-      HasVar x t1 ->
-      HasVar x <{t1; t2}>
+      has_var x t1 ->
+      has_var x <{t1; t2}>
 
   | hasvar_seq2 : forall t1 t2,
-      HasVar x t2 ->
-      HasVar x <{t1; t2}>
+      has_var x t2 ->
+      has_var x <{t1; t2}>
 
   | hasvar_spawn : forall t,
-      HasVar x t ->
-      HasVar x <{spawn t}>
+      has_var x t ->
+      has_var x <{spawn t}>
   .
 
-
-
-
-
-
-
-
-
-
-
-
-
-
-
-
-
-
-
-
-
-
-Ltac inversion_nomut :=
-  match goal with
-  | H : NoMut <{unit    }> |- _ => inversion H; subst
-  | H : NoMut <{N _     }> |- _ => inversion H; subst
-  | H : NoMut <{& _ :: _}> |- _ => inversion H; subst
-  | H : NoMut <{new _ _ }> |- _ => inversion H; subst
-  | H : NoMut <{* _     }> |- _ => inversion H; subst
-  | H : NoMut <{_ = _   }> |- _ => inversion H; subst
-  | H : NoMut <{var _   }> |- _ => inversion H; subst
-  | H : NoMut <{fn _ _ _}> |- _ => inversion H; subst
-  | H : NoMut <{call _ _}> |- _ => inversion H; subst
-  | H : NoMut <{_ ; _   }> |- _ => inversion H; subst
-  | H : NoMut <{spawn _ }> |- _ => inversion H; subst
-  end.
-
-Ltac inversion_clear_nomut :=
-  match goal with
-  | H : NoMut <{unit    }> |- _ => inv_clear H
-  | H : NoMut <{N _     }> |- _ => inv_clear H
-  | H : NoMut <{& _ :: _}> |- _ => inv_clear H
-  | H : NoMut <{new _ _ }> |- _ => inv_clear H
-  | H : NoMut <{* _     }> |- _ => inv_clear H
-  | H : NoMut <{_ = _   }> |- _ => inv_clear H
-  | H : NoMut <{var _   }> |- _ => inv_clear H
-  | H : NoMut <{fn _ _ _}> |- _ => inv_clear H
-  | H : NoMut <{call _ _}> |- _ => inv_clear H
-  | H : NoMut <{_ ; _   }> |- _ => inv_clear H
-  | H : NoMut <{spawn _ }> |- _ => inv_clear H
-  end.
-
-Local Lemma nomut_subst : forall x t t',
-  NoMut t ->
-  NoMut t' ->
-  NoMut ([x := t'] t).
-Proof.
-  intros. induction t; intros;
-  inversion_nomut; eauto using NoMut;
-  simpl; destruct String.string_dec; subst; eauto using NoMut. 
-Qed.
-
-
-Ltac inversion_ss :=
-  match goal with
-  | H : SafeSpawns <{unit    }> |- _ => inversion H; subst
-  | H : SafeSpawns <{N _     }> |- _ => inversion H; subst
-  | H : SafeSpawns <{& _ :: _}> |- _ => inversion H; subst
-  | H : SafeSpawns <{new _ _ }> |- _ => inversion H; subst
-  | H : SafeSpawns <{* _     }> |- _ => inversion H; subst
-  | H : SafeSpawns <{_ = _   }> |- _ => inversion H; subst
-  | H : SafeSpawns <{var _   }> |- _ => inversion H; subst
-  | H : SafeSpawns <{fn _ _ _}> |- _ => inversion H; subst
-  | H : SafeSpawns <{call _ _}> |- _ => inversion H; subst
-  | H : SafeSpawns <{_ ; _   }> |- _ => inversion H; subst
-  | H : SafeSpawns <{spawn _ }> |- _ => inversion H; subst
-  end.
-
-Ltac inversion_clear_ss :=
-  match goal with
-  | H : SafeSpawns <{unit    }> |- _ => inv_clear H
-  | H : SafeSpawns <{N _     }> |- _ => inv_clear H
-  | H : SafeSpawns <{& _ :: _}> |- _ => inv_clear H
-  | H : SafeSpawns <{new _ _ }> |- _ => inv_clear H
-  | H : SafeSpawns <{* _     }> |- _ => inv_clear H
-  | H : SafeSpawns <{_ = _   }> |- _ => inv_clear H
-  | H : SafeSpawns <{var _   }> |- _ => inv_clear H
-  | H : SafeSpawns <{fn _ _ _}> |- _ => inv_clear H
-  | H : SafeSpawns <{call _ _}> |- _ => inv_clear H
-  | H : SafeSpawns <{_ ; _   }> |- _ => inv_clear H
-  | H : SafeSpawns <{spawn _ }> |- _ => inv_clear H
-  end.
-
-Ltac inversion_hv :=
-  match goal with
-  | H : HasVar _ <{unit    }> |- _ => inversion H; subst
-  | H : HasVar _ <{N _     }> |- _ => inversion H; subst
-  | H : HasVar _ <{& _ :: _}> |- _ => inversion H; subst
-  | H : HasVar _ <{new _ _ }> |- _ => inversion H; subst
-  | H : HasVar _ <{* _     }> |- _ => inversion H; subst
-  | H : HasVar _ <{_ = _   }> |- _ => inversion H; subst
-  | H : HasVar _ <{var _   }> |- _ => inversion H; subst
-  | H : HasVar _ <{fn _ _ _}> |- _ => inversion H; subst
-  | H : HasVar _ <{call _ _}> |- _ => inversion H; subst
-  | H : HasVar _ <{_ ; _   }> |- _ => inversion H; subst
-  | H : HasVar _ <{spawn _ }> |- _ => inversion H; subst
-  end.
-
-Ltac inversion_clear_hv :=
-  match goal with
-  | H : HasVar _ <{unit    }> |- _ => inv_clear H
-  | H : HasVar _ <{N _     }> |- _ => inv_clear H
-  | H : HasVar _ <{& _ :: _}> |- _ => inv_clear H
-  | H : HasVar _ <{new _ _ }> |- _ => inv_clear H
-  | H : HasVar _ <{* _     }> |- _ => inv_clear H
-  | H : HasVar _ <{_ = _   }> |- _ => inv_clear H
-  | H : HasVar _ <{var _   }> |- _ => inv_clear H
-  | H : HasVar _ <{fn _ _ _}> |- _ => inv_clear H
-  | H : HasVar _ <{call _ _}> |- _ => inv_clear H
-  | H : HasVar _ <{_ ; _   }> |- _ => inv_clear H
-  | H : HasVar _ <{spawn _ }> |- _ => inv_clear H
-  end.
-
-Lemma hasvar_dec : forall x t,
-  Decidable.decidable (HasVar x t).
-Proof.
-  unfold Decidable.decidable. intros. induction t;
-  try (destruct IHt); try (destruct IHt1); try (destruct IHt2);
-  try match goal with
-    | x : id, x' : id |- _ =>
-      destruct (String.string_dec x x'); subst
-  end;
-  solve
-    [ left; eauto using HasVar
-    | right; intros F; inv_clear F; eauto; contradiction
-    ].
-Qed.
-
-Local Ltac solve_not_hasvar :=
-  intros; match goal with
-  | |- (~ HasVar _ ?t) => induction t; eauto using HasVar
-  end.
-
-Lemma not_hv_new : forall x t T,
-  ~ HasVar x <{new T t}> -> ~ HasVar x t.
-Proof. solve_not_hasvar. Qed.
-
-Lemma not_hv_load : forall x t,
-  ~ HasVar x <{*t}> -> ~ HasVar x t.
-Proof. solve_not_hasvar. Qed.
-
-Lemma not_hv_asg1 : forall x t1 t2,
-  ~ HasVar x <{t1 = t2}> -> ~ HasVar x t1.
-Proof. solve_not_hasvar. Qed.
-
-Lemma not_hv_asg2 : forall x t1 t2,
-  ~ HasVar x <{t1 = t2}> -> ~ HasVar x t2.
-Proof. solve_not_hasvar. Qed.
-
-Lemma not_hv_fun : forall x x' t Tx,
-  x <> x' -> ~ HasVar x <{fn x' Tx t}> -> ~ HasVar x t.
-Proof. solve_not_hasvar. Qed.
-
-Lemma not_hv_call1 : forall x t1 t2,
-  ~ HasVar x <{call t1 t2}> -> ~ HasVar x t1.
-Proof. solve_not_hasvar. Qed.
-
-Lemma not_hv_call2 : forall x t1 t2,
-  ~ HasVar x <{call t1 t2}> -> ~ HasVar x t2.
-Proof. solve_not_hasvar. Qed.
-
-Lemma not_hv_seq1 : forall x t1 t2,
-  ~ HasVar x <{t1; t2}> -> ~ HasVar x t1.
-Proof. solve_not_hasvar. Qed.
-
-Lemma not_hv_seq2 : forall x t1 t2,
-  ~ HasVar x <{t1; t2}> -> ~ HasVar x t2.
-Proof. solve_not_hasvar. Qed.
-
-Lemma not_hv_spawn : forall x t,
-  ~ HasVar x <{spawn t}> -> ~ HasVar x t.
-Proof. solve_not_hasvar. Qed.
-
-Lemma hasvar_subst : forall x t tx,
-  ~ (HasVar x t) -> ([x := tx] t) = t.
-Proof.
-  intros. induction t; simpl; trivial;
-  try (destruct String.string_dec; subst; trivial);
-  solve
-    [ rewrite IHt; eauto using not_hv_new, not_hv_load, not_hv_spawn, not_hv_fun
-    | rewrite IHt1; eauto using not_hv_asg1, not_hv_call1, not_hv_seq1;
-      rewrite IHt2; eauto using not_hv_asg2, not_hv_call2, not_hv_seq2
-    | exfalso; eauto using HasVar
-    ].
-Qed.
-
-Lemma hasvar_typing : forall Gamma x t T,
-  HasVar x t ->
-  Gamma x = None ->
-  ~ (Gamma |-- t is T).
-Proof.
-  assert (forall Gamma x, Gamma x = None -> (safe Gamma) x = None).
-  { unfold safe. intros * H. rewrite H. reflexivity. }
-  intros * ? HGamma F. induction_type; inversion_hv; eauto.
-  - rewrite HGamma in *. discriminate.
-  - rewrite lookup_update_neq in IHF; eauto.
-Qed.
-
 (* ------------------------------------------------------------------------- *)
-(* Equivalence                                                               *)
+(* no-mut inversion                                                          *)
 (* ------------------------------------------------------------------------- *)
 
-Local Lemma equivalence_safe : forall Gamma1 Gamma2,
-  Gamma1 === Gamma2 ->
-  safe Gamma1 === safe Gamma2.
-Proof.
-  unfold map_equivalence, safe. intros * Heq k.
-  specialize (Heq k). rewrite Heq. trivial.
-Qed.
+Local Ltac match_nomut tactic :=
+  match goal with
+  (* irrelevant for unit      *)
+  (* irrelevant for num       *)
+  | H : no_mut <{& _ :: Unit     }> |- _ => tactic H
+  | H : no_mut <{& _ :: Num      }> |- _ => tactic H
+  (* irrelevant if &ad :: i&T *)
+  | H : no_mut <{& _ :: & _      }> |- _ => tactic H
+  | H : no_mut <{& _ :: (_ --> _)}> |- _ => tactic H
+  | H : no_mut <{new _ _         }> |- _ => tactic H
+  | H : no_mut <{* _             }> |- _ => tactic H
+  | H : no_mut <{_ = _           }> |- _ => tactic H
+  (* irrelevant for var       *)
+  | H : no_mut <{fn _ _ _        }> |- _ => tactic H
+  | H : no_mut <{call _ _        }> |- _ => tactic H
+  | H : no_mut <{_ ; _           }> |- _ => tactic H
+  | H : no_mut <{spawn _         }> |- _ => tactic H
+  end.
 
-Local Lemma equivalence_typing : forall Gamma1 Gamma2 t T,
-  Gamma1 === Gamma2 ->
-  Gamma1 |-- t is T ->
-  Gamma2 |-- t is T.
-Proof.
-  intros. generalize dependent Gamma2. induction_type; intros;
-  eauto using type_of, equivalence_safe,
-    MapEquivalence.lookup, MapEquivalence.update_equivalence.
-Qed.
+Ltac inv_nomut := match_nomut inv.
+
+Ltac invc_nomut := match_nomut invc.
+
+(* ------------------------------------------------------------------------- *)
+(* safe-spawns inversion                                                     *)
+(* ------------------------------------------------------------------------- *)
+
+Local Ltac match_ss tactic :=
+  match goal with
+  (* irrelevant for unit *)
+  (* irrelevant for num  *)
+  (* irrelevant for ad   *)
+  | H : safe_spawns <{new _ _ }> |- _ => tactic H
+  | H : safe_spawns <{* _     }> |- _ => tactic H
+  | H : safe_spawns <{_ = _   }> |- _ => tactic H
+  (* irrelevant for var  *)
+  | H : safe_spawns <{fn _ _ _}> |- _ => tactic H
+  | H : safe_spawns <{call _ _}> |- _ => tactic H
+  | H : safe_spawns <{_ ; _   }> |- _ => tactic H
+  | H : safe_spawns <{spawn _ }> |- _ => tactic H
+  end.
+
+Ltac inv_ss := match_ss inv.
+
+Ltac invc_ss := match_ss invc.
+
+(* ------------------------------------------------------------------------- *)
+(* has-var inversion                                                         *)
+(* ------------------------------------------------------------------------- *)
+
+Local Ltac match_hv tactic :=
+  match goal with
+  | H : has_var _   <{unit    }> |- _ => tactic H
+  | H : has_var _   <{N _     }> |- _ => tactic H
+  | H : has_var _   <{& _ :: _}> |- _ => tactic H
+  | H : has_var _   <{new _ _ }> |- _ => tactic H
+  | H : has_var _   <{* _     }> |- _ => tactic H
+  | H : has_var _   <{_ = _   }> |- _ => tactic H
+  | H : has_var ?x1 <{var ?x2 }> |- _ => tactic H
+  | H : has_var _   <{fn _ _ _}> |- _ => tactic H
+  | H : has_var _   <{call _ _}> |- _ => tactic H
+  | H : has_var _   <{_ ; _   }> |- _ => tactic H
+  | H : has_var _   <{spawn _ }> |- _ => tactic H
+  end.
+
+Ltac inv_hv := match_hv inv.
+
+Ltac invc_hv := match_hv invc.
 
