Definitions.v
@@ -1,6 +1,9 @@
 From Elo Require Export ValidAddresses.
 From Elo Require Export WellTypedTerm.
-From Elo Require Export ConsistentlyTypedReferences.
+From Elo Require Export CTR.
 From Elo Require Export Access.
 From Elo Require Export NotAccess.
 From Elo Require Export UnsafeAccess.
+From Elo Require Export SafeSpawns.
+From Elo Require Export SMS.
+
