PropertiesCTR.v
@@ -1,0 +1,308 @@
+From Elo Require Import Util.
+From Elo Require Import Array.
+From Elo Require Import Map.
+From Elo Require Import Core.
+From Elo Require Import CoreExt.
+
+From Elo Require Import Definitions.
+
+(* ------------------------------------------------------------------------- *)
+(* preservation                                                              *)
+(* ------------------------------------------------------------------------- *)
+
+Module Preservation.
+
+  (* auxiliary. *)
+  Local Lemma step_write_wtt : forall m t t' ad v Tr T,
+    empty |-- t is T ->
+    t --[EF_Write ad v Tr]--> t' ->
+    consistently_typed_references m t ->
+    (Tr = m[ad].typ /\ exists V, empty |-- v is V /\ empty |-- m[ad].tm is V).
+  Proof.
+    intros * ? ?.
+    assert (exists V, empty |-- v is V) as [? ?].
+    { generalize dependent T. induction_tstep; intros; inv_type; eauto. }
+    intros. generalize dependent T.
+    induction_tstep; intros; inv_type; inv_ctr; eauto.
+    inv_type. inv_ctr. apply_deterministic_typing. eauto.
+  Qed.
+
+  (* subst & mem ----------------------------------------------------------- *)
+
+  Lemma ctr_subst_preservation : forall m t tx x,
+    consistently_typed_references m t ->
+    consistently_typed_references m tx ->
+    consistently_typed_references m ([x := tx] t).
+  Proof.
+    intros. induction t; trivial;
+    try solve [inv_ctr; eauto using consistently_typed_references];
+    simpl; destruct string_eq_dec; subst; trivial.
+    inv_ctr. eauto using consistently_typed_references.
+  Qed.
+
+  Lemma ctr_mem_add_preservation : forall m t vT,
+    valid_addresses m t ->
+    consistently_typed_references m t ->
+    consistently_typed_references (m +++ vT) t.
+  Proof.
+    intros. induction t; eauto using consistently_typed_references;
+    inv_vad; inv_ctr; eauto using consistently_typed_references;
+    (eapply ctr_refM || eapply ctr_refI); simpl_array; assumption.
+  Qed.
+
+  Lemma ctr_mem_set_preservation : forall m t ad v T,
+    ad < #m ->
+    empty |-- v is T ->
+    empty |-- m[ad].tm is T ->
+    (* --- *)
+    consistently_typed_references m t ->
+    consistently_typed_references m[ad <- (v, m[ad].typ)] t.
+  Proof.
+    intros. induction t;
+    eauto using consistently_typed_references;
+    inv_ctr; eauto using consistently_typed_references;
+    match goal with _ : _[?ad].typ = _ |- _ => rename ad into ad' end;
+    (eapply ctr_refM || eapply ctr_refI);
+    decompose sum (lt_eq_lt_dec ad' ad); subst;
+    simpl_array; trivial; apply_deterministic_typing; trivial.
+  Qed.
+
+  (* tstep ----------------------------------------------------------------- *)
+
+  Lemma ctr_tstep_none_preservation : forall m t t',
+    consistently_typed_references m t ->
+    t --[EF_None]--> t' ->
+    consistently_typed_references m t'.
+  Proof.
+    intros. induction_tstep; inv_ctr; eauto using consistently_typed_references.
+    inv_ctr. eauto using ctr_subst_preservation.
+  Qed.
+
+  Local Lemma ctr_tstep_alloc_preservation : forall m t t' v T,
+    valid_addresses m t ->
+    well_typed_term t ->
+    (* --- *)
+    consistently_typed_references m t ->
+    t --[EF_Alloc (#m) v T]--> t' ->
+    consistently_typed_references (m +++ (v, T)) t'.
+  Proof.
+    intros * ? [T' ?] **. generalize dependent T'.
+    induction_tstep; intros; inv_vad; inv_type; inv_ctr;
+    eauto using consistently_typed_references, ctr_mem_add_preservation;
+    (eapply ctr_refM || eapply ctr_refI); simpl_array; trivial.
+  Qed.
+
+  Local Lemma ctr_tstep_read_preservation : forall m t t' ad v,
+    consistently_typed_references m v ->
+    consistently_typed_references m t ->
+    t --[EF_Read ad v]--> t' ->
+    consistently_typed_references m t'.
+  Proof.
+    intros. induction_tstep; inv_ctr;
+    eauto using consistently_typed_references.
+  Qed.
+
+  Local Lemma ctr_tstep_write_preservation : forall m t t' ad v T,
+    well_typed_term t ->
+    valid_addresses m t ->
+    consistently_typed_references m t ->
+    t --[EF_Write ad v T]--> t' ->
+    consistently_typed_references m[ad <- (v, T)] t'.
+  Proof.
+    intros * [T' ?]. intros. assert (
+      T = m[ad].typ /\
+      exists Tv, empty |-- v is Tv /\ empty |-- m[ad].tm is Tv)
+      as [? [? [? ?]]] by eauto using step_write_wtt.
+    generalize dependent T'.
+    induction_tstep; intros; inv_type; inv_vad; inv_ctr;
+    eauto using valid_address_write,
+      consistently_typed_references,
+      ctr_mem_set_preservation.
+  Qed.
+
+  Lemma ctr_tstep_spawn_preservation : forall m t t' block,
+    consistently_typed_references m t ->
+    t --[EF_Spawn block]--> t' ->
+    consistently_typed_references m t'.
+  Proof.
+    intros. induction_tstep; inv_ctr;
+    eauto using consistently_typed_references.
+  Qed.
+
+  Local Corollary ctr_mstep_preservation : forall m m' t t' e,
+    well_typed_term t ->
+    valid_addresses m t ->
+    forall_memory m (consistently_typed_references m) ->
+    consistently_typed_references m t ->
+    m / t ==[e]==> m' / t' ->
+    consistently_typed_references m' t'.
+  Proof.
+    solve_mstep_preservation_using
+      ctr_tstep_none_preservation
+      ctr_tstep_alloc_preservation
+      ctr_tstep_read_preservation
+      ctr_tstep_write_preservation.
+  Qed.
+
+  (* ------------------------------------------------------------------------- *)
+
+  Local Lemma ctr_thread_default_preservation : forall m,
+    consistently_typed_references m thread_default.
+  Proof.
+    eauto using consistently_typed_references.
+  Qed.
+
+  Lemma ctr_spawn_block : forall m t t' block,
+    consistently_typed_references m t ->
+    t --[EF_Spawn block]--> t' ->
+    consistently_typed_references m block.
+  Proof.
+    intros. induction_tstep; inv_ctr; eauto.
+  Qed.
+
+  Local Lemma ctr_untouched_threads_preservation : forall m m' ths tid tid' e t',
+    forall_threads ths well_typed_term ->
+    forall_threads ths (valid_addresses m) ->
+    forall_threads ths (consistently_typed_references m) ->
+    tid <> tid' ->
+    tid' < #ths ->
+    m / ths[tid] ==[e]==> m' / t' ->
+    consistently_typed_references m' ths[tid'].
+  Proof.
+    intros *. intros Htype. intros. destruct (Htype tid).
+    inv_mstep; eauto using ctr_mem_add_preservation.
+    match goal with
+    | _ : _ --[EF_Write _ _ ?T]--> _ |- _ =>
+      assert (
+        T = m[ad].typ /\
+        exists V, empty |-- v is V /\ empty |-- m[ad].tm is V)
+        as [Heq [? [? ?]]] by eauto using step_write_wtt
+    end.
+    rewrite Heq in *. eauto using ctr_mem_set_preservation.
+  Qed.
+
+  Corollary ctr_cstep_preservation : forall m m' ths ths' tid e,
+    forall_threads ths well_typed_term ->
+    forall_threads ths (valid_addresses m) ->
+    forall_memory m (consistently_typed_references m) ->
+    forall_threads ths (consistently_typed_references m) ->
+    m / ths ~~[tid, e]~~> m' / ths' ->
+    forall_threads ths' (consistently_typed_references m').
+  Proof.
+    intros * Htype ?. destruct (Htype tid).
+    eauto 6 using cstep_preservation,
+      ctr_tstep_spawn_preservation,
+      ctr_mstep_preservation,
+      ctr_thread_default_preservation,
+      ctr_spawn_block,
+      ctr_untouched_threads_preservation.
+  Qed.
+
+(* ------------------------------------------------------------------------- *)
+
+Local Lemma wtt_alloc_value_generalization : forall t t' ad v T,
+  well_typed_term t ->
+  t --[EF_Alloc ad v T]--> t' ->
+  well_typed_term v.
+Proof.
+  unfold well_typed_term. intros * [T' ?]. intros. generalize dependent T'.
+  induction_tstep; intros; inv_type; eauto.
+Qed.
+
+Local Lemma ctr_alloc_value_generalization : forall m t t' ad v T,
+  consistently_typed_references m t ->
+  t --[EF_Alloc ad v T]--> t' ->
+  consistently_typed_references m v.
+Proof.
+  intros. induction_tstep; intros; inv_ctr; eauto.
+Qed.
+
+Local Lemma ctr_write_value_generalization : forall m t t' ad v T,
+  consistently_typed_references m t ->
+  t --[EF_Write ad v T]--> t' ->
+  consistently_typed_references m v.
+Proof.
+  intros. induction_tstep; intros; inv_ctr; eauto.
+Qed.
+
+Local Lemma ctr_tstep_alloc_mem_preservation : forall m t t' v T,
+  well_typed_term t ->
+  valid_addresses m t ->
+  forall_memory m (valid_addresses m) ->
+  (* --- *)
+  consistently_typed_references m t ->
+  forall_memory m (consistently_typed_references m) ->
+  t --[EF_Alloc (#m) v T]--> t' ->
+  forall_memory (m +++ (v, T)) (consistently_typed_references (m +++ (v, T))).
+Proof.
+  intros. intros ad.
+  assert (well_typed_term v) as [? ?]
+    by eauto using wtt_alloc_value_generalization.
+  decompose sum (lt_eq_lt_dec ad (#m)); subst; simpl_array;
+  eauto using consistently_typed_references; (* optimization *)
+  eauto using ctr_mem_add_preservation, ctr_alloc_value_generalization.
+Qed.
+
+Local Lemma ctr_tstep_write_mem_preservation : forall m t t' ad v T,
+  ad < # m ->
+  well_typed_term t ->
+  (* --- *)
+  consistently_typed_references m t ->
+  forall_memory m (consistently_typed_references m) ->
+  t --[EF_Write ad v T]--> t' ->
+  forall_memory m[ad <- (v, T)] (consistently_typed_references m[ad <- (v, T)]).
+Proof.
+  intros * ? [? ?]. intros. intros ad'.
+  match goal with
+  | _ : _ --[EF_Write _ _ ?T]--> _ |- _ =>
+    assert (
+      T = m[ad].typ /\
+      exists V, empty |-- v is V /\ empty |-- m[ad].tm is V)
+      as [? [? [? ?]]] by eauto using step_write_wtt
+  end.
+  decompose sum (lt_eq_lt_dec ad' ad); subst; simpl_array;
+  eauto using ctr_write_value_generalization, ctr_mem_set_preservation.
+Qed.
+
+Local Corollary ctr_mstep_mem_preservation : forall m m' t t' e,
+  well_typed_term t ->
+  valid_addresses m t ->
+  forall_memory m (valid_addresses m) ->
+  (* --- *)
+  consistently_typed_references m t ->
+  forall_memory m (consistently_typed_references m) ->
+  m / t ==[e]==> m' / t' ->
+  forall_memory m' (consistently_typed_references m').
+Proof.
+  solve_mstep_mem_preservation_using 
+    ctr_tstep_alloc_mem_preservation 
+    ctr_tstep_write_mem_preservation.
+Qed.
+
+Local Corollary ctr_cstep_mem_preservation : forall m m' ths ths' tid e,
+  forall_threads ths well_typed_term ->
+  forall_threads ths (valid_addresses m) ->
+  forall_memory m (valid_addresses m) ->
+  (* --- *)
+  forall_threads ths (consistently_typed_references m) ->
+  forall_memory m (consistently_typed_references m) ->
+  m / ths ~~[tid, e]~~> m' / ths' ->
+  forall_memory m' (consistently_typed_references m').
+Proof.
+  solve_cstep_mem_preservation_using ctr_mstep_mem_preservation.
+Qed.
+
+(* ------------------------------------------------------------------------- *)
+
+Theorem consistently_typed_references_preservation : forall m m' ths ths' tid e,
+  forall_program m ths well_typed_term ->
+  forall_program m ths (valid_addresses m) ->
+  (* --- *)
+  forall_program m ths (consistently_typed_references m) ->
+  m / ths ~~[tid, e]~~> m' / ths' ->
+  forall_program m' ths' (consistently_typed_references m').
+Proof.
+  intros * [_ ?] [? ?] [? ?]. intros.
+  eauto using ctr_cstep_preservation, ctr_cstep_mem_preservation.
+Qed.
+
