PropertiesVAD.v
@@ -1,0 +1,256 @@
+From Elo Require Import Util.
+From Elo Require Import Array.
+From Elo Require Import Core.
+From Elo Require Import CoreExt.
+
+From Elo Require Import AnyTerm.
+From Elo Require Import Meta.
+
+From Elo Require Import Definitions.
+
+(* ------------------------------------------------------------------------- *)
+(* valid-addresses implies valid-accesses                                    *)
+(* ------------------------------------------------------------------------- *)
+
+Local Lemma acc_then_hasad : forall m t ad,
+  access ad m t ->
+  t has_address ad \/ (exists ad', m[ad'].tm has_address ad).
+Proof.
+  intros * Hacc. induction Hacc; try decompose [or and] IHHacc;
+  eauto using anyt, is_address.
+Qed.
+
+Lemma vad_then_vac : forall m t,
+  forall_memory m (valid_addresses m) ->
+  valid_addresses m t ->
+  valid_accesses m t.
+Proof.
+  intros * Hmvad ? ? Hacc. autounfold with vad in Hmvad.
+  eapply acc_then_hasad in Hacc as [? | [? ?]]; eauto.
+Qed.
+
+Lemma mvad_then_mvac : forall m,
+  forall_memory m (valid_addresses m) ->
+  forall_memory m (valid_accesses m).
+Proof.
+  intros * Hmvad ? ? Hacc. autounfold with vad in Hmvad.
+  eapply acc_then_hasad in Hacc as [? | [? ?]]; eauto.
+Qed.
+
+Corollary forall_program_vad_then_vac : forall m ths,
+  forall_program m ths (valid_addresses m) ->
+  forall_program m ths (valid_accesses m).
+Proof.
+  intros * [? ?]; split; eauto using mvad_then_mvac.
+  intros ?. eauto using vad_then_vac.
+Qed.
+
+(* ------------------------------------------------------------------------- *)
+(* preservation                                                              *)
+(* ------------------------------------------------------------------------- *)
+
+Module Preservation.
+
+  (* subst & mem ----------------------------------------------------------- *)
+
+  Lemma vad_subst_preservation : forall m t tx x,
+    valid_addresses m t ->
+    valid_addresses m tx ->
+    valid_addresses m ([x := tx] t).
+  Proof.
+    intros.
+    induction t; trivial; simpl; try solve [inv_vad; eauto with vad];
+    destruct string_eq_dec; subst; trivial. inv_vad. eauto with vad.
+  Qed.
+
+  Lemma vad_mem_add_preservation : forall m t vT,
+    valid_addresses m t ->
+    valid_addresses (m +++ vT) t.
+  Proof.
+    intros. induction t; eauto with vad; inv_vad; eauto with vad.
+    intros ? ?. inv_hasad. rewrite add_increments_length. eauto.
+  Qed.
+
+  Lemma vad_mem_set_preservation : forall m t ad vT,
+    valid_addresses m t ->
+    valid_addresses m[ad <- vT] t.
+  Proof.
+    intros. induction t; eauto with vad; inv_vad; eauto with vad.
+    intros ? ?. inv_hasad. rewrite set_preserves_length. assumption.
+  Qed.
+
+  (* tstep ----------------------------------------------------------------- *)
+
+  Lemma vad_tstep_none_preservation : forall m t t',
+    valid_addresses m t ->
+    t --[EF_None]--> t' ->
+    valid_addresses m t'.
+  Proof.
+    intros. induction_tstep; inv_vad; eauto with vad. 
+    inv_vad. eauto using vad_subst_preservation.
+  Qed.
+
+  Lemma vad_tstep_alloc_preservation : forall m t t' v T,
+    valid_addresses m t ->
+    t --[EF_Alloc (#m) v T]--> t' ->
+    valid_addresses (m +++ (v, T)) t'.
+  Proof.
+    intros. induction_tstep; inv_vad;
+    eauto using vad_mem_add_preservation with vad.
+    intros ? ?. inv_hasad. rewrite add_increments_length. eauto.
+  Qed.
+
+  Lemma vad_tstep_read_preservation : forall m t t' ad v,
+    valid_addresses m v ->
+    valid_addresses m t ->
+    t --[EF_Read ad v]--> t' ->
+    valid_addresses m t'.
+  Proof.
+    intros. induction_tstep; inv_vad; eauto with vad.
+  Qed.
+
+  Lemma vad_tstep_write_preservation : forall m t t' ad v T,
+    valid_addresses m t ->
+    t --[EF_Write ad v T]--> t' ->
+    valid_addresses m[ad <- (v, T)] t'.
+  Proof.
+    intros. induction_tstep; inv_vad;
+    eauto using vad_mem_set_preservation with vad.
+  Qed.
+
+  Lemma vad_tstep_spawn_preservation : forall m t t' block,
+    valid_addresses m t ->
+    t --[EF_Spawn block]--> t' ->
+    valid_addresses m t'.
+  Proof.
+    intros. induction_tstep; inv_vad; eauto with vad.
+  Qed.
+
+  (* mstep ----------------------------------------------------------------- *)
+
+  Corollary vad_mstep_preservation : forall m m' t t' e,
+    forall_memory m (valid_addresses m) ->
+    valid_addresses m t ->
+    m / t ==[e]==> m' / t' ->
+    valid_addresses m' t'.
+  Proof.
+    intros. inv_mstep;
+    eauto using vad_tstep_none_preservation,
+                vad_tstep_alloc_preservation,
+                vad_tstep_read_preservation,
+                vad_tstep_write_preservation.
+  Qed.
+
+  (* cstep ----------------------------------------------------------------- *)
+
+  Lemma vad_thread_default : forall m,
+    valid_addresses m thread_default.
+  Proof.
+    intros. eauto with vad.
+  Qed.
+
+  Lemma vad_spawn_block : forall m t t' block,
+    valid_addresses m t ->
+    t --[EF_Spawn block]--> t' ->
+    valid_addresses m block.
+  Proof.
+    intros. induction_tstep; inv_vad; eauto.
+  Qed.
+
+  Lemma vad_untouched_threads_preservation : forall m m' ths tid tid' t' e,
+    forall_threads ths (valid_addresses m) ->
+    tid <> tid' ->
+    tid' < #ths ->
+    m / ths[tid] ==[e]==> m' / t' ->
+    valid_addresses m' ths[tid'].
+  Proof.
+    intros. inv_mstep; 
+    eauto using vad_mem_add_preservation, vad_mem_set_preservation.
+  Qed.
+
+  Corollary vad_cstep_preservation : forall m m' ths ths' tid e,
+    forall_program m ths (valid_addresses m) ->
+    m / ths ~~[tid, e]~~> m' / ths' ->
+    forall_threads ths' (valid_addresses m').
+  Proof.
+    intros. eauto 6 using cstep_preservation,
+      vad_tstep_spawn_preservation,
+      vad_mstep_preservation,
+      vad_thread_default,
+      vad_spawn_block,
+      vad_untouched_threads_preservation.
+  Qed.
+
+  (* tstep mem ------------------------------------------------------------- *)
+
+  Lemma vad_tstep_alloc_mem_preservation : forall m t t' v T,
+    forall_memory m (valid_addresses m) ->
+    valid_addresses m t ->
+    t --[EF_Alloc (#m) v T]--> t' ->
+    forall_memory  (m +++ (v, T)) (valid_addresses (m +++ (v, T))).
+  Proof.
+    assert (forall m t t' ad v T,
+      valid_addresses m t ->
+      t --[EF_Alloc ad v T]--> t' ->
+      valid_addresses m v)
+        by (intros; induction_tstep; inv_vad; eauto).
+    (* main proof *)
+    intros ** ad.
+    decompose sum (lt_eq_lt_dec ad (#m)); subst; simpl_array;
+    eauto using vad_mem_add_preservation with vad.
+  Qed.
+
+  Lemma vad_tstep_write_mem_preservation : forall m t t' ad v T,
+    forall_memory m (valid_addresses m) ->
+    valid_addresses m t ->
+    t --[EF_Write ad v T]--> t' ->
+    forall_memory m[ad <- (v, T)] (valid_addresses m[ad <- (v, T)]).
+  Proof.
+    assert (forall m t t' ad v T,
+      valid_addresses m t ->
+      t --[EF_Write ad v T]--> t' ->
+      valid_addresses m v)
+        by (intros; induction_tstep; inv_vad; eauto).
+    (* main proof *)
+    intros ** ad'.
+    assert (ad < #m)
+      by (intros; induction_tstep; inv_vad; eauto; inv_vad; assumption).
+    destruct (nat_eq_dec ad ad'); subst; simpl_array;
+    eauto using vad_mem_set_preservation.
+  Qed.
+
+  (* mstep mem ------------------------------------------------------------- *)
+
+  Corollary vad_mstep_mem_preservation : forall m m' t t' e,
+    forall_memory m (valid_addresses m) ->
+    valid_addresses m t ->
+    m / t ==[e]==> m' / t' ->
+    forall_memory m' (valid_addresses m').
+  Proof.
+    intros. inv_mstep;
+    eauto using vad_tstep_alloc_mem_preservation,
+                vad_tstep_write_mem_preservation.
+  Qed.
+
+  (* cstep mem ------------------------------------------------------------- *)
+
+  Corollary vad_cstep_mem_preservation : forall m m' ths ths' tid e,
+    forall_program m ths (valid_addresses m) ->
+    m / ths ~~[tid, e]~~> m' / ths' ->
+    forall_memory m' (valid_addresses m').
+  Proof.
+    intros * [? ?] ?. inv_cstep; eauto using vad_mstep_mem_preservation.
+  Qed.
+
+  (* valid-addresses preservation ------------------------------------------ *)
+
+  Theorem valid_addresses_preservation : forall m m' ths ths' tid e,
+    forall_program m ths (valid_addresses m) ->
+    m / ths ~~[tid, e]~~> m' / ths' ->
+    forall_program m' ths' (valid_addresses m').
+  Proof.
+    eauto using vad_cstep_preservation, vad_cstep_mem_preservation.
+  Qed.
+
+End Preservation.
+
