SmsPreservation.v
@@ -1,0 +1,213 @@
+
+(* ------------------------------------------------------------------------- *)
+(* acc, uacc & memtyp                                                        *)
+(* ------------------------------------------------------------------------- *)
+
+(* If the access is unsafe, then the memtyp is mutable. *)
+Local Lemma uacc_then_memtyp_mut : forall m t ad,
+  forall_memory m (consistently_typed_references m) ->
+  consistently_typed_references m t ->
+  (* --- *)
+  unsafe_access ad m t ->
+  exists T, m[ad].typ = <{{&T}}>.
+Proof.
+  intros * ? ? Huacc. induction Huacc; inversion_ctr; eauto.
+Qed.
+
+(* If the memtyp is mutable, then the access is unsafe. *)
+Local Lemma memtyp_mut_then_uacc : forall m t ad T,
+  forall_memory m value ->
+  forall_memory m (consistently_typed_references m) ->
+  consistently_typed_references m t ->
+  (* --- *)
+  m[ad].typ = <{{&T}}> ->
+  access ad m t ->
+  unsafe_access ad m t.
+Proof.
+  intros * ? ? ? Heq Hacc.
+  induction Hacc; inversion_ctr; eauto using unsafe_access.
+  - exfalso. eauto using immutable_reference_then_nuacc.
+  - rewrite Heq in *. discriminate.
+Qed.
+
+(* If one access is unsafe, then all accesses are unsafe. *)
+Local Corollary uacc_from_association : forall m t t' ad,
+  forall_memory m value ->
+  forall_memory m (consistently_typed_references m) ->
+  consistently_typed_references m t ->
+  consistently_typed_references m t' ->
+  (* --- *)
+  access ad m t ->
+  unsafe_access ad m t' ->
+  unsafe_access ad m t.
+Proof.
+  intros.
+  assert (exists T, m[ad].typ = <{{&T}}>) as [? ?];
+  eauto using uacc_then_memtyp_mut, memtyp_mut_then_uacc.
+Qed.
+
+(* ------------------------------------------------------------------------- *)
+(* preservation                                                              *)
+(* ------------------------------------------------------------------------- *)
+
+Local Lemma step_write_sms_helper : forall m t ad v ths tid tid' T,
+  tid <> tid' ->
+  forall_threads ths well_typed_term ->
+  safe_memory_sharing m ths ->
+  ths[tid] --[EF_Write ad v T]--> t ->
+  ~ access ad m ths[tid'].
+Proof.
+  assert (forall m t t' ad v T Te,
+    empty |-- t is T ->
+    t --[EF_Write ad v Te]--> t' ->
+    unsafe_access ad m t
+  ). {
+    intros. generalize dependent T.
+    induction_step; intros; inversion_type; eauto using unsafe_access.
+    inversion_type. eauto using unsafe_access.
+  }
+  (* main proof *)
+  intros * Hneq Htype Hsms ? Hacc.
+  destruct (Htype tid). specialize (Hsms _ _ _ Hneq Hacc); eauto.
+Qed.
+
+(* tstep ------------------------------------------------------------------- *)
+
+(*
+  Three cases:
+  - needs nuacc-tstep-preservation;
+  - needs acc-tstep-inheritance;
+  - just safe-memory-sharing.
+*)
+
+Local Ltac destruct_sms ths tid tid1 tid2 :=
+  assert (Hlt : tid < #ths) by eauto using step_length_tid;
+  destruct (nat_eq_dec tid tid1), (nat_eq_dec tid tid2); subst;
+  try contradiction.
+
+Local Lemma sms_tstep_none_preservation : forall m t ths tid,
+  safe_memory_sharing m ths ->
+  ths[tid] --[EF_None]--> t ->
+  safe_memory_sharing m ths[tid <- t].
+Proof.
+  intros ** tid1 tid2 **. destruct_sms ths tid tid1 tid2; simpl_array;
+  eauto using acc_tstep_none_inheritance, nuacc_tstep_none_preservation.
+Qed.
+
+Local Lemma sms_tstep_alloc_preservation : forall m t v ths tid T,
+  forall_memory m (valid_addresses m) ->
+  forall_threads ths (valid_addresses m) ->
+  (* --- *)
+  safe_memory_sharing m ths ->
+  ths[tid] --[EF_Alloc (#m) v T]--> t ->
+  safe_memory_sharing (m +++ (v, T)) ths[tid <- t].
+Proof.
+  intros ** tid1 tid2 ** Huacc.
+  assert (Hvac : forall_threads ths (valid_accesses m))
+    by eauto using forall_threads_vad_then_vac.
+  assert (forall tid, ~ unsafe_access (#m) m ths[tid])
+    by (intros * F; eapply uacc_then_acc in F; eapply Hvac in F; eauto).
+  autounfold with vac in Hvac. 
+  eapply uacc_then_acc in Huacc as ?. contradict Huacc.
+  destruct_sms ths tid tid1 tid2; simpl_array;
+  eauto 7 using nuacc_tstep_alloc_preservation,
+                acc_tstep_alloc_inheritance,
+                nuacc_mem_add_preservation,
+                acc_mem_add_inheritance.
+Qed.
+
+Local Lemma sms_tstep_read_preservation : forall m t ad ths tid,
+  forall_memory m value ->
+  forall_threads ths well_typed_term ->
+  forall_threads ths (consistently_typed_references m) ->
+  (* --- *)
+  safe_memory_sharing m ths ->
+  ths[tid] --[EF_Read ad m[ad].tm]--> t ->
+  safe_memory_sharing m ths[tid <- t].
+Proof.
+  intros * ? Hwtt ** tid1 tid2 **. destruct (Hwtt tid1).
+  destruct_sms ths tid tid1 tid2; simpl_array;
+  eauto using acc_tstep_read_inheritance, nuacc_tstep_read_preservation.
+Qed.
+
+Local Lemma sms_tstep_write_preservation : forall m ths t tid ad v T,
+  forall_threads ths well_typed_term ->
+  (* --- *)
+  safe_memory_sharing m ths ->
+  ths[tid] --[EF_Write ad v T]--> t ->
+  safe_memory_sharing m[ad <- (v, T)] ths[tid <- t].
+Proof.
+  intros ** tid1 tid2 ** Huacc.
+  eapply uacc_then_acc in Huacc as ?. contradict Huacc.
+  destruct_sms ths tid tid1 tid2; simpl_array;
+  try assert (~ access ad m ths[tid1]) by eauto using step_write_sms_helper;
+  try assert (~ access ad m ths[tid2]) by eauto using step_write_sms_helper;
+  eauto 7 using uacc_then_acc,
+    nuacc_tstep_write_preservation,
+    acc_tstep_write_inheritance,
+    alt_nuacc_mem_set_preservation,
+    alt_acc_mem_set_inheritance.
+Qed.
+
+Local Lemma sms_tstep_spawn_preservation : forall m ths t block tid,
+  forall_memory m value ->
+  forall_memory m (valid_addresses m) ->
+  forall_memory m (consistently_typed_references m) ->
+  forall_threads ths (valid_addresses m) ->
+  forall_threads ths (consistently_typed_references m) ->
+  forall_threads ths SafeSpawns ->
+  (* --- *)
+  safe_memory_sharing m ths ->
+  ths[tid] --[EF_Spawn block]--> t ->
+  safe_memory_sharing m (ths[tid <- t] +++ block).
+Proof.
+  intros ** tid1 tid2 **.
+  assert (~ unsafe_access ad m block) by eauto using nuacc_spawn_block .
+  assert (consistently_typed_references m block) by eauto using ctr_spawn_block.
+  destruct_sms ths tid tid1 tid2;
+  decompose sum (lt_eq_lt_dec tid1 (#ths)); subst; simpl_array;
+  decompose sum (lt_eq_lt_dec tid2 (#ths)); subst; simpl_array;
+  try solve [inversion_step | inv_acc | intros ?; inv_uacc];
+  eauto using uacc_from_association,
+    nuacc_tstep_spawn_preservation,
+    acc_tstep_spawn_inheritance.
+Qed.
+
+Local Corollary sms_mstep_preservation : forall m m' t e ths tid,
+  forall_memory m value ->
+  forall_memory m (valid_addresses m) ->
+  forall_threads ths (valid_addresses m) ->
+  forall_threads ths well_typed_term ->
+  forall_threads ths (consistently_typed_references m) ->
+  (* --- *)
+  safe_memory_sharing m ths ->
+  m / ths[tid] ==[e]==> m' / t ->
+  safe_memory_sharing m' ths[tid <- t].
+Proof.
+  intros. inversion_mstep;
+  eauto using sms_tstep_none_preservation,
+    sms_tstep_alloc_preservation,
+    sms_tstep_read_preservation,
+    sms_tstep_write_preservation.
+Qed.
+
+(* ------------------------------------------------------------------------- *)
+
+Theorem safe_memory_sharing_preservation : forall m m' ths ths' tid e,
+  forall_memory m value ->
+  forall_program m ths (valid_addresses m) ->
+  forall_program m ths well_typed_term ->
+  forall_program m ths (consistently_typed_references m) ->
+  forall_program m ths SafeSpawns ->
+  (* --- *)
+  safe_memory_sharing m ths ->
+  m / ths ~~[tid, e]~~> m' / ths' ->
+  safe_memory_sharing m' ths'.
+Proof.
+  intros * ? [? ?] [_ ?] [? ?] [_ ?] **.
+  assert (forall_threads ths (valid_accesses m))
+    by eauto using forall_threads_vad_then_vac.
+  inversion_clear_cstep;
+  eauto using sms_tstep_spawn_preservation, sms_mstep_preservation.
+Qed.
+
